thys/LLL_Basis_Reduction/Cost.thy
@@ -16,4 +16,13 @@ definition result :: "'a cost \<Rightarrow> 'a" where "result = fst"
 lemma cost_simps: "cost (a,c) = c" "result (a,c) = a" 
   unfolding cost_def result_def by auto
 
+lemma result_costD: assumes "result f_c = f" 
+  "cost f_c \<le> b"
+  "f_c = (a,c)"
+shows "a = f" "c \<le> b" using assms by (auto simp: cost_simps)
+
+lemma result_costD': assumes "result f_c = f \<and> cost f_c \<le> b"
+  "f_c = (a,c)"
+  shows "a = f" "c \<le> b" using assms by (auto simp: cost_simps)
+
 end
