thys/LLL_Basis_Reduction/LLL_Number_Bounds.thy
@@ -1033,6 +1033,28 @@ qed
 text \<open>Now we have bounds on each number $(f_i)_j$, $(g_i)_j$, and $\mu_{i,j}$, i.e.,
   for rational numbers bounds on the numerators and denominators.\<close>
 
+lemma logA_le_2log_Mn: assumes m: "m \<noteq> 0" "n \<noteq> 0" and A: "A > 0" 
+  shows "log 2 A \<le> 2 * log 2 (M * n)" 
+proof -
+  have "A \<le> nat M * nat M * n * 1" using A_le_MMn m by auto
+  also have "\<dots> \<le> nat M * nat M * n * n" by (intro mult_mono, insert m, auto)
+  finally have AM: "A \<le> nat M * nat M * n * n" by simp
+  with A have "nat M \<noteq> 0" by auto
+  hence M: "M > 0" by simp
+
+  have "log 2 A \<le> log 2 (M * M * n * n)" 
+  proof (subst log_le_cancel_iff)      
+    show "real A \<le> (M * M * int n * int n)" using AM[folded of_nat_le_iff[where ?'a = real]] M
+      by simp
+  qed (insert A M m, auto)
+  also have "\<dots> = log 2 (of_int (M * n) * of_int (M * n))" 
+    unfolding of_int_mult by (simp  add: ac_simps)
+  also have "\<dots> = 2 * log 2 (M * n)" 
+    by (subst log_mult, insert m M, auto)
+  finally show "log 2 A \<le> 2 * log 2 (M * n)" by auto
+qed
+
+
 text \<open>We now prove a combined size-bound for all of these numbers. The bounds clearly indicate
   that the size of the numbers grows at most polynomial, namely the sizes are roughly 
   bounded by ${\cal O}(m \cdot \log(M \cdot n))$ where $m$ is the number of vectors, $n$ is the dimension
@@ -1100,28 +1122,10 @@ proof -
     by (rule arg_cong[of _ _ "log 2"], subst powr_realpow, insert A, auto) 
   also have "\<dots> = (2 * m) * log 2 A" 
     by (subst log_powr, insert A, auto)
-  also have "log 2 (2^m) = m" by simp
-  finally show boundA: "log 2 \<bar>number\<bar> \<le> 2 * m * log 2 A + m + log 2 m" .
-  have "A \<le> nat M * nat M * n * 1" using A_le_MMn i by auto
-  also have "\<dots> \<le> nat M * nat M * n * n" by (intro mult_mono, insert j, auto)
-  finally have AM: "A \<le> nat M * nat M * n * n" by simp
-  with A have "nat M \<noteq> 0" by auto
-  hence M: "M > 0" by simp
-  note boundA
-  also have "2 * m * log 2 A + m + log 2 m \<le> 2 * m * (2 * log 2 (M * n)) + m + log 2 m" 
-  proof (intro add_right_mono mult_left_mono)
-    have "log 2 A \<le> log 2 (M * M * n * n)" 
-    proof (subst log_le_cancel_iff)      
-      show "real A \<le> (M * M * int n * int n)" using AM[folded of_nat_le_iff[where ?'a = real]] M
-        by simp
-    qed (insert A M j, auto)
-    also have "\<dots> = log 2 (of_int (M * n) * of_int (M * n))" 
-      unfolding of_int_mult by (simp  add: ac_simps)
-    also have "\<dots> = 2 * log 2 (M * n)" 
-      by (subst log_mult, insert j M, auto)
-    finally show "log 2 A \<le> 2 * log 2 (M * n)" .
-  qed auto
-  finally show "log 2 \<bar>number\<bar> \<le> 4 * m * log 2 (M * n) + m + log 2 m" by simp    
+  finally show boundA: "log 2 \<bar>number\<bar> \<le> 2 * m * log 2 A + m + log 2 m" by simp
+  also have "\<dots> \<le> 2 * m * (2 * log 2 (M * n)) + m + log 2 m" 
+    by (intro add_right_mono mult_mono logA_le_2log_Mn A, insert i j A, auto)
+  finally show "log 2 \<bar>number\<bar> \<le> 4 * m * log 2 (M * n) + m + log 2 m" by simp
 qed
 
 text \<open>And a combined size bound for an integer implementation which stores values 
@@ -1132,16 +1136,19 @@ lemma combined_size_bound_integer:
     \<union> {d\<mu> fs i j | i j. j < i \<and> i < m} 
     \<union> {d fs i | i. i \<le> m}" 
     (is "x \<in> ?fs \<union> ?d\<mu> \<union> ?d")
-  and m: "m \<noteq> 0" 
-shows "abs x \<le> A ^ (2 * m) * 2 ^ m * m" (* this is not tight, one could add a few -1 *)
+  and m: "m \<noteq> 0" and n: "n \<noteq> 0" 
+shows "abs x \<le> A ^ (2 * m) * 2 ^ m * m"
+  "x \<noteq> 0 \<Longrightarrow> log 2 \<bar>x\<bar> \<le> 2 * m * log 2 A       + m + log 2 m" (is "_ \<Longrightarrow> ?l1 \<le> ?b1")
+  "x \<noteq> 0 \<Longrightarrow> log 2 \<bar>x\<bar> \<le> 4 * m * log 2 (M * n) + m + log 2 m" (is "_ \<Longrightarrow> _ \<le> ?b2")
 proof -
   let ?bnd = "int A ^ (2 * m) * 2 ^ m * int m" 
   from bound_invD[OF binv]
   have inv: "LLL_invariant upw k fs"
      and fbnd: "f_bound outside k fs" 
      and gbnd: "g_bound fs" 
-    by auto
+    by auto 
   from LLL_inv_A_pos[OF inv gbnd m] have A: "A > 0" by auto
+  let ?r = real_of_int
   from x consider (fs) "x \<in> ?fs" | (d\<mu>) "x \<in> ?d\<mu>" | (d) "x \<in> ?d" by auto
   hence "abs x \<le> ?bnd" 
   proof cases
@@ -1169,7 +1176,19 @@ proof -
       by (intro mult_mono pow_mono_exp, insert A m, auto)
     finally show ?thesis .
   qed
-  thus ?thesis by simp
+  thus "abs x \<le> A ^ (2 * m) * 2 ^ m * m" by simp
+  hence abs: "?r (abs x) \<le> ?r (A ^ (2 * m) * 2 ^ m * m)" by linarith
+  assume "x \<noteq> 0" hence x: "abs x > 0" by auto
+  from abs have "log 2 (abs x) \<le> log 2 (?r (A ^ (2 * m)) * 2 ^ m * ?r m)" 
+    by (subst log_le_cancel_iff, insert x A m, auto)
+  also have "\<dots> = log 2 (?r A ^ (2 * m)) + m + log 2 (?r m)" 
+    using A m by (auto simp: log_mult)
+  also have "log 2 (?r A ^ (2 * m)) = real (2 * m) * log 2 (?r A)" 
+    by (subst log_nat_power, insert A, auto)
+  finally show "?l1 \<le> ?b1" by simp
+  also have "\<dots> \<le> 2 * m * (2 * log 2 (M * n)) + m + log 2 m" 
+    by (intro add_right_mono mult_left_mono logA_le_2log_Mn, insert m n A, auto)
+  finally show "?l1 \<le> ?b2" by simp  
 qed
 end (* LLL_bound_invariant *)
   
